theories/input_lang/interp.v
@@ -33,23 +33,18 @@ Defined.
 Section constructors.
   Context {E : opsInterp}.
   Context {subEff0 : subEff ioE E}.
-  Notation IT := (IT E).
-  Notation ITV := (ITV E).
+  Notation IT := (IT E natO).
+  Notation ITV := (ITV E natO).
 
-  Definition INPUT : (nat -n> IT) -n> IT.
-  Proof using E subEff0.
-    simple refine (λne k, Vis (E:=E) (subEff_opid (inl ()))
-                            (subEff_ins (F:=ioE) (op:=(inl ())) ())
-                            (NextO ◎ k ◎ (subEff_outs (F:=ioE) (op:=(inl ())))^-1)).
-    solve_proper.
-  Defined.
-  Definition OUTPUT_ : nat -n> IT -n> IT.
-  Proof using E subEff0.
-    simple refine (λne m α, Vis (E:=E) (subEff_opid (inr (inl ())))
+  Program Definition INPUT : (nat -n> IT) -n> IT := λne k, Vis (E:=E) (subEff_opid (inl ()))
+                                                             (subEff_ins (F:=ioE) (op:=(inl ())) ())
+                                                             (NextO ◎ k ◎ (subEff_outs (F:=ioE) (op:=(inl ())))^-1).
+  Solve Obligations with solve_proper.
+  Program Definition OUTPUT_ : nat -n> IT -n> IT :=
+    λne m α, Vis (E:=E) (subEff_opid (inr (inl ())))
                         (subEff_ins (F:=ioE) (op:=(inr (inl ()))) m)
-                        (λne _, NextO α)).
-    all: solve_proper_please.
-  Defined.
+                        (λne _, NextO α).
+  Solve All Obligations with solve_proper_please.
   Definition OUTPUT : nat -n> IT.
   Proof using E subEff0.
     simple refine (λne m, OUTPUT_ m (Nat 0)).
@@ -77,8 +72,8 @@ Section weakestpre.
   Variable (rs : gReifiers sz).
   Context {subR : subReifier reify_io rs}.
   Notation F := (gReifiers_ops rs).
-  Notation IT := (IT F).
-  Notation ITV := (ITV F).
+  Notation IT := (IT F natO).
+  Notation ITV := (ITV F natO).
   Context `{!invGS Σ, !stateG rs Σ}.
   Notation iProp := (iProp Σ).
 
@@ -98,7 +93,7 @@ Section weakestpre.
   Lemma wp_output (σ σ' : stateO) (n : nat) Φ s :
     update_output n σ = σ' →
     has_substate σ -∗
-    ▷ (£ 1 -∗ has_substate σ' -∗ Φ (NatV 0)) -∗
+    ▷ (£ 1 -∗ has_substate σ' -∗ Φ (RetV 0)) -∗
     WP@{rs} (OUTPUT n) @ s {{ Φ }}.
   Proof.
     intros Hs. iIntros "Hs Ha".
@@ -117,14 +112,14 @@ Section interp.
   Variable (rs : gReifiers sz).
   Context {subR : subReifier reify_io rs}.
   Notation F := (gReifiers_ops rs).
-  Notation IT := (IT F).
-  Notation ITV := (ITV F).
+  Notation IT := (IT F natO).
+  Notation ITV := (ITV F natO).
 
   (** Interpreting individual operators *)
   Program Definition interp_input {A} : A -n> IT :=
     λne env, INPUT Nat.
   Program Definition interp_output {A} (t : A -n> IT) : A -n> IT :=
-    get_nat OUTPUT ◎ t.
+    get_ret OUTPUT ◎ t.
   Local Instance interp_ouput_ne {A} : NonExpansive2 (@interp_output A).
   Proof. solve_proper. Qed.
 
@@ -441,7 +436,7 @@ Section interp.
     head_step e σ e' σ' (n,0) →
     interp_expr e env ≡ Tick_n n $ interp_expr e' env.
   Proof.
-    inversion 1; cbn-[IF APP' INPUT Tick get_nat2].
+    inversion 1; cbn-[IF APP' INPUT Tick get_ret2].
     - (*fun->val*)
       reflexivity.
     - (* app lemma *)
@@ -464,7 +459,7 @@ Section interp.
     - (* the natop stuff *)
       simplify_eq.
       destruct v1,v2; try naive_solver. simpl in *.
-      rewrite NATOP_Nat.
+      rewrite NATOP_Ret.
       destruct op; simplify_eq/=; done.
     - by rewrite IF_True.
     - rewrite IF_False; eauto. lia.
@@ -509,7 +504,7 @@ Section interp.
       by rewrite ofe_iso_21.
     - trans (reify (gReifiers_sReifier rs) (interp_ectx K env (OUTPUT n0)) (gState_recomp σr (sR_state σ))).
       { do 3 f_equiv; eauto.
-        rewrite get_nat_nat//. }
+        rewrite get_ret_ret//. }
       trans (reify (gReifiers_sReifier rs) (OUTPUT_ n0 (interp_ectx K env (Nat 0))) (gState_recomp σr (sR_state σ))).
       { do 2 f_equiv; eauto.
         rewrite hom_OUTPUT_//. }
@@ -549,7 +544,7 @@ Section interp.
         eauto.
       + eapply (interp_expr_fill_yes_reify K env _ _ _ _ σr) in H2.
         rewrite interp_ectx_fill. simpl.
-        rewrite get_nat_nat.
+        rewrite get_ret_ret.
         rewrite hom_OUTPUT_.
         change 1 with (1+0). econstructor; last first.
         { apply ssteps_zero; reflexivity. }
@@ -560,7 +555,7 @@ Section interp.
         rewrite -H2.
         repeat f_equiv; eauto.
         Opaque OUTPUT_.
-        rewrite interp_ectx_fill /= get_nat_nat hom_OUTPUT_.
+        rewrite interp_ectx_fill /= get_ret_ret hom_OUTPUT_.
         eauto.
   Qed.
 
